Examples

Examples.v
@@ -7,9 +7,9 @@ Open Scope string.
 
 Definition empty_graph := G<>G.
 Definition test_graph := G<
-    -( 1 "person" [("name", VStr "Alice"); ("age", VNum 23)] )-;
-    -( 2 "person" [("name", VStr "Bob"); ("age", VNum 24)] )-;
-    -( 3 "person" [("name", VStr "Charlie"); ("age", VNum 30)] )-;
+    -( 1 "person" [("name", VStr "Alice"); ("age", VNum 23); ("marital status", VStr "married")] )-;
+    -( 2 "person" [("name", VStr "Bob"); ("age", VNum 24); ("marital status", VStr "single")])-;
+    -( 3 "person" [("name", VStr "Charlie"); ("age", VNum 30); ("marital status", VStr "married")] )-;
     -( 4 "organization" [("name", VStr "Google"); ("area", VStr "technology")] )-;
     -( 5 "organization" [("name", VStr "Microsoft"); ("area", VStr "technology")] )-;
     -( 6 "organization" [("name", VStr "University of Maryland"); ("area", VStr "education")] )-;
@@ -17,13 +17,13 @@ Definition test_graph := G<
     -( 8 "state" [("name", VStr "Washington")] )-;
     -( 9 "state" [("name", VStr "New York")] )-;
     -( 10 "state" [("name", VStr "Maryland")] )-;
-    -( 1 )--[ 1 "works_at" [] ]->-( 4 )-;
-    -( 1 )--[ 2 "from" [] ]->-( 9 )-;
+    -( 1 )--[ 1 "works_at" [("since", VNum 2018)] ]->-( 4 )-;
+    -( 1 )--[ 2 "from" [] ]->-( 10 )-;
     -( 1 )--[ 3 "studied_at" [] ]->-( 6 )-;
-    -( 2 )--[ 4 "works_at" [] ]->-( 4 )-;
-    -( 2 )--[ 5 "from" [] ]->-( 10 )-;
+    -( 2 )--[ 4 "works_at" [("since", VNum 2020)] ]->-( 4 )-;
+    -( 2 )--[ 5 "from" [] ]->-( 9 )-;
     -( 2 )--[ 6 "studied_at" [] ]->-( 7 )-;
-    -( 3 )--[ 7 "works_at" [] ]->-( 5 )-;
+    -( 3 )--[ 7 "works_at" [("since", VNum 2019)] ]->-( 5 )-;
     -( 3 )--[ 8 "from" [] ]->-( 8 )-;
     -( 3 )--[ 9 "studied_at" [] ]->-( 6 )-;
     -( 4 )--[ 10 "locates_in" [] ]->-( 9 )-;
@@ -32,17 +32,81 @@ Definition test_graph := G<
     -( 7 )--[ 13 "locates_in" [] ]->-( 8 )-
   >G.
 
-Compute (pattern_match test_graph 
-?? 
--( :"state" [] )- <-[ :: [] ]- -( :: [] )- 
--[ :: [] ]- -( :: [])-
-??).
 
-Compute (eval_expr test_graph [("org", VId (NodeId 7))] <{ "org"["area"] }>).
+(* Names and ages of all people ("Dummy" column is just to demonstrate constant projection ) *)
+Definition q_name_and_age := MATCH -( "p" :"person" [] )-
+                             RETURN <{ "p"["name"] }> AS "Name",
+                                    <{ "p"["age"] }> AS "Age",
+                                    <{ 1 + 1 }> AS "Dummy".
+Example q_name_and_age_ok : 
+  execute test_graph q_name_and_age = [
+    [("Name", VStr "Alice"); ("Age", VNum 23); ("Dummy", VNum 2)];
+    [("Name", VStr "Bob"); ("Age", VNum 24); ("Dummy", VNum 2)];
+    [("Name", VStr "Charlie"); ("Age", VNum 30); ("Dummy", VNum 2)]
+  ].
+Proof.
+  reflexivity.
+Qed.
 
-Definition test_paths := pattern_match test_graph test_pattern.
-Definition bound_test_paths := map (bind_path test_graph test_pattern) test_paths.
-Definition projected_table := project test_graph [(<{ "p"["name"] }>, "who");
-                                                  (<{ "s"["name"] }>, "where")]
-                                                 bound_test_paths.
-Compute (execute test_graph test_query).
+(* Names and workplaces of married people *)
+Definition q_workplace_of_married_people :=
+  MATCH -( "p" :"person" [("marital status", VStr "married")] )- -[ "w" :"works_at" [] ]-> -( "o" :"organization" [] )-
+  RETURN <{ "p"["name"] }> AS "Name",
+         <{ "o"["name"] }> AS "Company",
+         <{ 2022 - "w"["since"] }> AS "Years of work".
+Example q_workplace_of_married_people_ok:
+  execute test_graph q_workplace_of_married_people = [
+    [("Name", VStr "Alice"); ("Company", VStr "Google"); ("Years of work", VNum 4)];
+    [("Name", VStr "Charlie"); ("Company", VStr "Microsoft"); ("Years of work", VNum 3)]
+  ].
+Proof.
+  reflexivity.
+Qed.
+
+(* People and organizations from the state of Washington *)
+Definition q_from_Washington :=
+  MATCH -( :: [("name", VStr "Washington")] )- <-[ :"from":"locates_in" [] ]- -( "entity" :: [] )-
+  RETURN <{ "entity"["name"] }> AS "Name",
+         <{ "entity"["age"] }> AS "Age",
+         <{ "entity"["area"]}> AS "Area".
+Example q_from_Washington_ok:
+  execute test_graph q_from_Washington = [
+    [("Name", VStr "University of Washington"); ("Area", VStr "education")];
+    [("Name", VStr "Microsoft"); ("Area", VStr "technology")];
+    [("Name", VStr "Charlie"); ("Age", VNum 30)]
+  ].
+Proof.
+  reflexivity.
+Qed.
+
+(* People and the states they work in *)
+Definition q_people_work_in_states :=
+  MATCH -( "p" :"person" [] )- -[ "w" :"works_at" [] ]- -( "o" :: [] )- -[ :"locates_in" [] ]- -( "s" :: [] )-
+  RETURN <{ "p"["name"] }> AS "Name",
+         <{ "o"["name"] }> AS "Company",
+         <{ "s"["name"]}> AS "State",
+         <{ "w"["since"]}> AS "Since".
+Example q_people_work_in_states_ok :
+  execute test_graph q_people_work_in_states = [
+    [("Name", VStr "Alice"); ("Company", VStr "Google"); ("State", VStr "New York"); ("Since", VNum 2018)];
+    [("Name", VStr "Bob"); ("Company", VStr "Google"); ("State", VStr "New York"); ("Since", VNum 2020)];
+    [("Name", VStr "Charlie"); ("Company", VStr "Microsoft"); ("State", VStr "Washington"); ("Since", VNum 2019)]
+  ].
+Proof.
+  reflexivity.
+Qed.
+
+Definition q_people_work_and_come_from_the_same_state :=
+  MATCH -( "p" :"person" [] )- -[ :"works_at" [] ]-> 
+        -( :: [] )- -[ :"locates_in" [] ]-> 
+        -( "s" :: [] )- <-[ :"from" [] ]- -( "p" :"person" [])-
+  RETURN <{ "p"["name"] }> AS "Name",
+         <{ "s"["name"]}> AS "State".
+Example q_people_work_and_come_from_the_same_state_ok :
+  execute test_graph q_people_work_and_come_from_the_same_state = [
+    [("Name", VStr "Bob"); ("State", VStr "New York")];
+    [("Name", VStr "Charlie"); ("State", VStr "Washington")]
+  ].
+Proof.  
+  reflexivity.
+Qed.
